crypto/bignum/Hacl.Bignum.Crecip.fsti
@@ -1,0 +1,18 @@
+module Hacl.Bignum.Crecip
+
+
+open FStar.HyperStack
+open FStar.Buffer
+
+open Hacl.Bignum.Parameters
+open Hacl.Bignum.Bigint
+open Hacl.Bignum.Limb
+open Hacl.Bignum.Fproduct
+
+module U32 = FStar.UInt32
+
+val crecip:
+  out:felem ->
+  z:felem -> Stack unit
+  (requires (fun h -> live h out /\ live h z))
+  (ensures (fun h0 _ h1 -> live h1 out /\ modifies_1 out h0 h1))
