crypto/bignum/Hacl.Bignum.Parameters.fsti
@@ -15,6 +15,10 @@ inline_for_extraction let wide = if word_size = 32 then Hacl.UInt64.t else Hacl.
 inline_for_extraction let ctr  = FStar.UInt32.t
 
 
+val v: limb -> GTot nat
+val w: wide -> GTot nat
+
+
 (** Number of limbs of a bigint **)
 val len: pos
 inline_for_extraction val clen: l:FStar.UInt32.t{FStar.UInt32.v l = len}
@@ -24,15 +28,18 @@ type felem_wide = b:buffer wide{length b = len}
 
 
 (** Associates a weight in bits to each limb of the bigint *)
-val template: idx:nat{idx < len} -> Tot pos
-val ctemplate:
-  idx:FStar.UInt32.t{FStar.UInt32.v idx < len} ->
-  Tot (x:FStar.UInt32.t{template (FStar.UInt32.v idx) = FStar.UInt32.v x})
-
-
-(** Predicate associated to 'workable' bigintegers, restored after each bigint computation **)
-val reduced: h:mem -> b:felem -> Tot bool
-val reduced_wide: h:mem -> b:felem_wide -> Tot bool
+(* val template: idx:nat{idx < len} -> Tot pos *)
+(* val ctemplate: *)
+(*   idx:FStar.UInt32.t{FStar.UInt32.v idx < len} -> *)
+(*   Tot (x:FStar.UInt32.t{template (FStar.UInt32.v idx) = FStar.UInt32.v x}) *)
+val limb_size: pos
+inline_for_extraction val climb_size: l:FStar.UInt32.t{limb_size = FStar.UInt32.v l}
 
 (** Predicate associated to 'workable' bigintegers, restored after each bigint computation **)
-val reducible: h:mem -> b:felem -> Tot bool
+val reduced_after_mul: h:mem -> b:felem -> GTot Type0
+val reduced_before_mul_l: h:mem -> b:felem -> GTot Type0
+val reduced_before_mul_r: h:mem -> b:felem -> GTot Type0
+val reduced_wide: h:mem -> b:felem_wide -> GTot Type0
+
+(** Predicate associated to 'workable' bigintegers, restored after each bigint computation **)
+val reducible: h:mem -> b:felem -> GTot Type0
