crypto/bignum/Hacl.EC.AddAndDouble.fsti
@@ -1,0 +1,19 @@
+module Hacl.EC.AddAndDouble
+
+open FStar.Mul
+open FStar.HyperStack
+open FStar.Ghost
+open FStar.Buffer
+
+open Hacl.Bignum.Parameters
+open Hacl.EC.Point
+
+val fmonty:
+  pp:point ->
+  ppq:point ->
+  p:point ->
+  pq:point ->
+  q:point ->
+  Stack unit
+    (requires (fun _ -> true))
+    (ensures (fun _ _ _ -> true))
