crypto/bignum/Hacl.EC.Ladder.fst
@@ -1,0 +1,146 @@
+module Hacl.EC.Ladder
+
+
+open FStar.Mul
+open FStar.HyperStack
+open FStar.Ghost
+open FStar.Buffer
+
+
+open Hacl.Bignum.Parameters
+open Hacl.Bignum.Limb
+open Hacl.EC.Point
+open Hacl.EC.AddAndDouble
+
+
+module U32 = FStar.UInt32
+module H8 = Hacl.UInt8
+
+
+#set-options "--lax"
+
+type uint8_p = buffer H8.t
+
+
+val cmult_small_loop:
+  nq:point ->
+  nqpq:point ->
+  nq2:point ->
+  nqpq2:point ->
+  q:point ->
+  byte:H8.t ->
+  i:ctr ->  
+  (* nqx:felem -> nqz:felem -> nqpqx:felem -> nqpqz:felem -> *)
+  (* nqx2:felem -> nqz2:felem -> nqpqx2:felem -> nqpqz2:felem -> q:felem -> byte:H8.t -> *)
+  (* i:U32.t -> *)
+  Stack unit
+    (requires (fun h -> true))
+    (ensures (fun h0 _ h1 -> true))
+(* let rec cmult_small_loop nqx nqz nqpqx nqpqz nqx2 nqz2 nqpqx2 nqpqz2 q byte i = *)
+let rec cmult_small_loop nq nqpq nq2 nqpq2 q byte i =
+  let nqx = getx nq in
+  let nqz = getz nq in
+  let nqpqx = getx nqpq in
+  let nqpqz = getz nqpq in
+  let nqx2 = getx nq2 in
+  let nqz2 = getz nq2 in
+  let nqpqx2 = getx nqpq2 in
+  let nqpqz2 = getz nqpq2 in
+  if (U32 (i =^ 0ul)) then ()
+  else (
+    let bit = byte_to_limb (H8 (byte >>^ 7ul)) in
+    (* swap_conditional nqx nqpqx bit; *)
+    (* swap_conditional nqz nqpqz bit; *)
+    swap_conditional nq nqpq bit;
+    (* fmonty nqx2 nqz2 nqpqx2 nqpqz2 nqx nqz nqpqx nqpqz q; *)
+    fmonty nq2 nqpq2 nq nqpq q;
+    (* swap_conditional nqx2 nqpqx2 bit; *)
+    (* swap_conditional nqz2 nqpqz2 bit; *)
+    swap_conditional nq2 nqpq2 bit;
+    let t = nqx in
+    let nqx = nqx2 in
+    let nqx2 = t in
+    let t = nqz in
+    let nqz = nqz2 in
+    let nqz2 = t in
+    let t = nqpqx in
+    let nqpqx = nqpqx2 in
+    let nqpqx2 = t in
+    let t = nqpqz in
+    let nqpqz = nqpqz2 in
+    let nqpqz2 = t in
+    let byte = H8 (byte <<^ 1ul) in
+    (* cmult_small_loop nqx nqz nqpqx nqpqz nqx2 nqz2 nqpqx2 nqpqz2 q byte (U32 (i -^ 1ul)) *)
+    cmult_small_loop nq nqpq nq2 nqpq2 q byte (U32 (i -^ 1ul))
+  )
+
+
+val cmult_big_loop:
+  n:uint8_p{length n = 32} ->
+  (* nqx:felem -> nqz:felem -> *)
+  (* nqpqx:felem -> nqpqz:felem -> *)
+  (* nqx2:felem -> nqz2:felem -> *)
+  (* nqpqx2:felem -> nqpqz2:felem -> *)
+  nq:felem ->
+  nqpq:felem ->
+  nq2:felem ->
+  nqpq2:felem ->
+  q:felem -> i:U32.t ->
+  Stack unit
+    (requires (fun h -> true))
+    (ensures (fun h0 _ h1 -> true))
+(* let rec cmult_big_loop n nqx nqz nqpqx nqpqz nqx2 nqz2 nqpqx2 nqpqz2 q i = *)
+let rec cmult_big_loop n nq nqpq nq2 nqpq2 q i =
+  if (U32 (i =^ 0ul)) then ()
+  else (
+    let i = U32 (i -^ 1ul) in
+    let byte = n.(i) in
+    cmult_small_loop nq nqpq nq2 nqpq2 q byte 8ul;
+    cmult_big_loop n nq nqpq nq2 nqpq2 q i
+  )
+
+
+val cmult:
+  (* resultx:felem -> resultz:felem -> *)
+  result:felem ->
+  n:uint8_p{length n = 32} ->
+  q:felem ->
+  Stack unit
+    (requires (fun _ -> true))
+    (ensures (fun _ _ _ -> true))
+    (* (requires (fun h -> live h resultx /\ live h resultz /\ live h n /\ live h q)) *)
+    (* (ensures (fun h0 _ h1 -> modifies_2 resultx resultz h0 h1 /\ live h1 resultx /\ live h1 resultz)) *)
+let cmult result n q =
+  push_frame();
+  let buf = create zero 40ul in
+  (* let nqpqx  = Buffer.sub buf 0ul  5ul in *)
+  (* let nqpqz  = Buffer.sub buf 5ul  5ul in *)
+  (* let nqx    = Buffer.sub buf 10ul 5ul in *)
+  (* let nqz    = Buffer.sub buf 15ul 5ul in *)
+  (* let nqpqx2 = Buffer.sub buf 20ul 5ul in *)
+  (* let nqpqz2 = Buffer.sub buf 25ul 5ul in *)
+  (* let nqx2   = Buffer.sub buf 30ul 5ul in *)
+  (* let nqz2   = Buffer.sub buf 35ul 5ul in *)
+  let nqpq  = Buffer.sub buf 0ul  10ul in
+  let nq    = Buffer.sub buf 10ul 10ul in
+  let nqpq2 = Buffer.sub buf 20ul 10ul in
+  let nq2   = Buffer.sub buf 30ul 10ul in
+  let nqpqx = getx nqpq in
+  let nqpqz = getz nqpq in
+  let nqx = getx nq in
+  let nqz = getz nq in
+  let nqpqx2 = getx nqpq2 in
+  let nqpqz2 = getz nqpq2 in
+  let nqx2 = getx nq2 in
+  let nqz2 = getz nq2 in
+  nqpqz.(0ul) <- one;
+  nqx.(0ul) <- one;
+  nqpqz2.(0ul) <- one;
+  nqz2.(0ul) <- one;
+  blit q 0ul nqpqx 0ul 5ul;
+  (* cmult_big_loop n nqx nqz nqpqx nqpqz nqx2 nqz2 nqpqx2 nqpqz2 q 32ul; *)
+  cmult_big_loop n nq nqpq nq2 nqpq2 q 32ul;
+  copy result nq;
+  (* blit nqx 0ul resultx 0ul 5ul; *)
+  (* blit nqz 0ul resultz 0ul 5ul; *)
+  pop_frame()
