crypto/bignum/Hacl.EC.Point.fsti
@@ -1,0 +1,49 @@
+module Hacl.EC.Point
+
+open FStar.Mul
+open FStar.HyperStack
+open FStar.Ghost
+open FStar.Buffer
+
+open Hacl.Bignum.Parameters
+open Hacl.Bignum.Bigint
+open Hacl.Bignum.Limb
+open Hacl.Bignum
+
+module U32 = FStar.UInt32
+
+val plen: pos
+val cplen: x:U32.t{plen = U32.v x}
+
+let point : Type0 = b:buffer limb{length b = plen}
+
+(** Coordinate getters *)
+val getx: point -> Tot felem
+val gety: point -> Tot felem
+val getz: point -> Tot felem
+
+
+(** Liveness of the point, depends on the Jacobian/Projective setup **)
+val live_coords: mem -> felem -> felem -> felem -> GTot bool
+val live: mem -> point -> GTot bool
+
+val make: felem -> felem -> felem -> Tot point
+
+
+(** Workable state of a point **)
+val valid: mem -> point -> GTot bool
+
+val swap_conditional:
+  a:point ->
+  b:point ->
+  i:limb ->
+  Stack unit
+    (requires (fun _ -> true))
+    (ensures (fun _ _ _ -> true))
+
+val copy:
+  output:point ->
+  input:point ->
+  Stack unit
+    (requires (fun _ -> true))
+    (ensures (fun _ _ _ -> true))
