crypto/bignum/x25519/Hacl.Bignum.Parameters.fst
@@ -1,0 +1,43 @@
+module Hacl.Bignum.Parameters
+
+open FStar.HyperStack
+open FStar.Buffer
+
+let prime =
+  assert_norm (pow2 255 > 19);
+  pow2 255 - 19
+
+let word_size = 64
+
+let v x = Hacl.UInt64.v x
+let w x = Hacl.UInt128.v x
+
+let len = 5
+inline_for_extraction let clen = 5ul
+
+let limb_size = 51
+inline_for_extraction let climb_size = 51ul
+
+let reduced_after_mul h b =
+  let _ = 0 in
+  live h b /\ v (get h b 0) < pow2 52 /\ v (get h b 1) < pow2 52 /\ v (get h b 2) < pow2 52
+  /\ v (get h b 3) < pow2 52 /\ v (get h b 4) < pow2 52
+
+let reduced_before_mul_l h b =
+  let _ = 0 in
+  live h b /\ v (get h b 0) < pow2 53 /\ v (get h b 1) < pow2 53 /\ v (get h b 2) < pow2 53
+  /\ v (get h b 3) < pow2 53 /\ v (get h b 4) < pow2 53
+
+let reduced_before_mul_r h b =
+  let _ = 0 in
+  live h b /\ v (get h b 0) < pow2 54 /\ v (get h b 1) < pow2 54 /\ v (get h b 2) < pow2 54
+  /\ v (get h b 3) < pow2 54 /\ v (get h b 4) < pow2 54
+
+let reduced_wide h b =
+  let _ = 0 in
+  live h b /\ w (get h b 0) < pow2 52 /\ w (get h b 1) < pow2 52 /\ w (get h b 2) < pow2 52
+  /\ w (get h b 3) < pow2 52 /\ w (get h b 4) < pow2 52
+
+let reducible h b =
+  (* TODO *)
+  admit()
